Added an FSetInterface for VarSets. Enabled *some* automation for reasoning about VarSets. However, I also broke some proofs. Note that VarSets do *not* have exact equality --- they keep track of vars by their uniques, so two equal sets can store different vars as long as those vars have the same uniques. Adding some of this reasoning into our lemmas and such broke some of the later proofs.

examples/ghc/theories/CoreFVs.v
@@ -10,43 +10,192 @@ Require Import Proofs.Base.
 Require Import Proofs.CoreInduct.
 Require Import Proofs.Core.
 
+Require Import Proofs.VarSet.
+Import VarSetFSet.
+Import VarSetDecide.
+Import VarSetFacts.
+Import VarSetProperties.
+Import VarSetFSet.Notin.
+
+Require GHC.Base.
+Import GHC.Base.ManualNotations.
+
 Set Bullet Behavior "Strict Subproofs".
 
+(* TODO: fix mutual recursion. *)
 Axiom freeVarsBind1_freeVarsBind: freeVarsBind1 = freeVarsBind.
-
-Import GHC.Base.Notations.
 
 Scheme expr_mut := Induction for Expr Sort Prop
   with bind_mut := Induction for Bind Sort Prop.
 
-(** Basic properties of [exprFreeVars] *)
+(** ** [FV] *)
 
-Axiom exprFreeVars_Var: forall v, exprFreeVars (Mk_Var v) = unitVarSet v.
+Axiom unionFV_empty_right : forall fv, FV.unionFV fv FV.emptyFV = fv.
+Axiom unionFV_empty_left  : forall fv, FV.unionFV FV.emptyFV fv = fv.
 
-Axiom exprFreeVars_Lam:
+(** Unfolding tactics *)
+
+Ltac unfold_FV := 
+  repeat unfold Base.op_z2218U__, FV.filterFV, FV.fvVarSet, 
+       FV.unitFV, FV.fvVarListVarSet.
+
+
+(** ** [VarSet] *)
+
+Lemma elemVarSet_emptyVarSet : forall v, elemVarSet v emptyVarSet = false.
+fsetdec.
+Qed.
+
+
+Lemma delVarSet_elemVarSet_false : forall v set, 
+    elemVarSet v set = false -> delVarSet set v [=] set.
+intros.
+set_b_iff.
+apply remove_equal.
+auto.
+Qed.
+
+
+Lemma extendVarSet_elemVarSet_true : forall set v, 
+    elemVarSet v set = true -> extendVarSet set v [=] set.
+Proof. 
+  intros.
+  set_b_iff.
+  apply add_equal.
+  auto.
+Qed.
+
+Lemma delVarSet_extendVarSet : 
+  forall set v, 
+    elemVarSet v set = false -> 
+    (delVarSet (extendVarSet set v) v) [=] set.
+Proof.
+  intros.
+  set_b_iff.
+  apply remove_add.
+  auto.
+Qed.
+
+Lemma elemVarSet_extendVarSet :
+  forall set v0 v, 
+    elemVarSet v0 (extendVarSet set v) = true -> 
+    (elemVarSet v0 set = true) \/ (Var_as_DT.eqb v v0 = true).
+Proof.
+  intros.
+  set_b_iff.
+  rewrite add_iff in H.
+  tauto.
+Qed.
+
+
+Definition disjoint E F := inter E F [=] empty.
+
+
+Lemma pass_through_unitFV : forall f v vs1 have haveSet v0,
+  disjoint vs1 haveSet ->
+  ~ (In v haveSet) ->
+  Tuple.snd (FV.unitFV v0 f (add v vs1) (have, haveSet)) [=]
+  remove v (Tuple.snd (FV.unitFV v0 f vs1 (have, haveSet))).
+Proof. 
+  intros.
+  unfold FV.unitFV.
+  destruct (elemVarSet v0 (add v vs1)) eqn:HE.
+  destruct (elemVarSet v0 haveSet) eqn:HE1;
+    destruct (elemVarSet v0 vs1) eqn:HE2;
+    simpl;
+    set_b_iff;
+    try fsetdec.  
+  + rewrite remove_equal; fsetdec.
+  + rewrite remove_equal; fsetdec.
+  + rewrite remove_equal; fsetdec.
+  + destruct (f v0); simpl.
+    assert (Var_as_DT.eqb v v0 = true). fsetdec.
+    admit. (* variant of remove_add *)
+    rewrite remove_equal; fsetdec.
+  + set_b_iff.
+    destruct_notin.
+    destruct (elemVarSet v0 vs1) eqn:HE2;
+      set_b_iff; try contradiction.
+    rewrite remove_equal.
+    fsetdec.
+    destruct (elemVarSet v0 haveSet) eqn: HE1.
+    auto.
+    destruct (f v0); simpl.
+    set_b_iff.
+    admit. (* seems like solve_notin should work here. *)
+    auto.
+Admitted.
+
+(** ** [expr_fvs] *)
+Lemma pass_through : forall e f v vs1 acc res1 res2,
+    disjoint vs1 (snd acc) ->
+    ~ (In v (snd acc)) ->
+    expr_fvs e f (add v vs1) acc = res1 ->
+    expr_fvs e f vs1         acc = res2 ->
+    snd res1 [=] remove v (snd res2).
+
+Proof.
+  intros e f v vs1.
+  apply (core_induct e); intros; unfold expr_fvs in *; simpl.
+  - subst. destruct acc. rewrite pass_through_unitFV. fsetdec.
+    simpl; auto. simpl; auto.
+Admitted.
+
+  (** Basic properties of [exprFreeVars] *)
+
+Lemma exprFreeVars_Var: forall v, 
+    isLocalVar v = true -> 
+    exprFreeVars (Mk_Var v) = unitVarSet v.
+Proof.
+intros v NG.
+unfold exprFreeVars, exprFVs, expr_fvs.
+unfold_FV.
+set_b_iff.
+rewrite NG.
+auto.
+Qed.
+
+Lemma exprFreeVars_Lam:
   forall v e,
   exprFreeVars (Lam v e) = delVarSet (exprFreeVars e) v.
+Proof.
+  intros.
+  unfold exprFreeVars, exprFVs.
+  unfold_FV.
+  unfold expr_fvs. fold expr_fvs.
+  unfold addBndr.
+  unfold varTypeTyCoFVs.
+  rewrite unionFV_empty_left.
+  unfold FV.delFV.
+  simpl.
+Admitted.
 
+
+
+  
 Lemma exprFreeVars_mkLams:
   forall vs e,
   exprFreeVars (mkLams vs e) = delVarSetList (exprFreeVars e) vs.
 Proof.
-  intros. 
+  intros.
+  set_b_iff.
   induction vs.
-  - unfold mkLams. unfold_Foldable.
-    unfold delVarSetList.
-    unfold UniqSet.delListFromUniqSet.
-    unfold UniqFM.delListFromUFM.
-    destruct (exprFreeVars e).
-    f_equal.
+  - unfold mkLams. 
+    unfold_Foldable_foldr.
+    unfold_Foldable_foldl.
+    simpl.
+    fsetdec.
   - revert IHvs.
     unfold mkLams.
-    unfold_Foldable.
-    unfold exprFreeVars.
-    unfold Base.op_z2218U__.
-    unfold exprFVs.
-    unfold Base.op_z2218U__.
+    unfold_Foldable_foldr.
     simpl.
+    rewrite exprFreeVars_Lam.
+    set_b_iff.
+    intro h.
+    rewrite h.
+    unfold_Foldable_foldl.
+    simpl.
+    set_b_iff.
 Admitted.
 
 (** Working with [freeVars] *)
@@ -80,10 +229,10 @@ Proof.
         simpl. do 2 f_equal.
         -- f_equal. erewrite <- H with (v:=c). reflexivity. intuition.
         -- assert (forall (v : CoreBndr) (rhs : Expr CoreBndr),
-                      In (v, rhs) l -> deAnnotate (freeVars rhs) = rhs).
+                      List.In (v, rhs) l -> deAnnotate (freeVars rhs) = rhs).
            { intros. apply H with (v:=v).
              apply in_cons; assumption. }
-           specialize (IHl H0 l2 l3 eq_refl). inversion IHl; reflexivity.
+           specialize (IHl H0 l2 l3 Logic.eq_refl). inversion IHl; reflexivity.
   - destruct (List.unzip
                 (List.map
                    (fun '(con, args, rhs) =>
@@ -147,7 +296,7 @@ Proof.
       rewrite reverse_append in IH.
       auto.
   }       
-  pose (K := H vs nil (length vs) eq_refl).
+  pose (K := H vs nil (length vs) Logic.eq_refl).
   simpl in K.
   auto.
 Qed.
