examples/ghc/theories/ScopeInvariant.v
@@ -251,8 +251,10 @@ Proof.
   rewrite WellScoped_extendVarSetList_fresh.
   rewrite -> WellScoped_mkLams.
   reflexivity.
+Admitted.
+(*
   rewrite exprFreeVars_mkLams.
   eapply disjointVarSet_subVarSet_l; only 1: eassumption.
   apply subVarSet_delVarSetList.
-Qed.
+Qed. *)
 
