examples/ghc/theories/VarSet.v
@@ -2,6 +2,9 @@ Require Import GHC.Base.
 Require Import CoreFVs.
 Require Import Id.
 Require Import Core.
+Require UniqFM.
+
+Import GHC.Base.ManualNotations.
 
 Require Import Proofs.GHC.Base.
 Require Import Proofs.GHC.List.
@@ -12,24 +15,122 @@ Require Import Coq.NArith.BinNat.
 
 Import ListNotations.
 
+Require Import Proofs.GhcTactics.
+Require Import Proofs.Unique.
+Require Import Proofs.Var.
+
+
+Require Import Proofs.Base.
+Require Import Proofs.ContainerAxioms.
+Require Import IntSetProofs. 
+(* Require Import IntMapProofs. *)
+
+Require Import Proofs.VarSetFSet.
+
+Import VarSetFSet.VarSetFacts.
+
 Open Scope Z_scope.
 
 Set Bullet Behavior "Strict Subproofs".
 
-Require Import Proofs.GhcTactics.
-Require Import Proofs.Base.
-Require Import Proofs.ContainerAxioms.
-Require Import Proofs.Unique.
-Require Import Proofs.Var.
-
-Require Import IntSetProofs.
-(* Require Import IntMapProofs. *)
-
 
 (** ** [VarSet] *)
 
+
+Lemma delVarSet_remove : forall x s, delVarSet s x = remove x s.
+tauto. Qed.
+
+Lemma extendVarSet_add : forall x s, extendVarSet s x = add x s.
+tauto. Qed.
+
+Lemma unitVarSet_singleton : forall x, unitVarSet x = singleton x.
+auto. Qed.
+
+Lemma extendVarSetList_foldl' : forall x xs, 
+    extendVarSetList x xs = 
+    Foldable.foldl' (fun x y => add y x) x xs.
+Proof.
+  intros.
+  unfold extendVarSetList,
+         UniqSet.addListToUniqSet;
+  replace UniqSet.addOneToUniqSet with 
+      (fun x y => add y x).
+  auto.
+  auto.
+Qed.
+
+Lemma delVarSetList_foldl : forall vl vs,
+    delVarSetList vs vl = Foldable.foldl delVarSet vs vl.
+Proof. 
+  induction vl.
+  - intro vs. 
+    unfold delVarSetList.
+    unfold UniqSet.delListFromUniqSet.
+    destruct vs.
+    unfold UniqFM.delListFromUFM.
+    unfold_Foldable_foldl.
+    simpl.
+    auto.
+  - intro vs. 
+    unfold delVarSetList in *.
+    unfold UniqSet.delListFromUniqSet in *.
+    destruct vs.
+    unfold UniqFM.delListFromUFM in *.
+    revert IHvl.
+    unfold_Foldable_foldl.
+    simpl.
+    intro IHvl.
+    rewrite IHvl with (vs:= (UniqSet.Mk_UniqSet (UniqFM.delFromUFM u a))).
+    auto.
+Qed.
+
+Lemma mkVarSet_extendVarSetList : forall xs,
+    mkVarSet xs = extendVarSetList emptyVarSet xs.
+Proof.
+  reflexivity.
+Qed.
+
+
+Ltac rewrite_extendVarSetList := 
+  unfold extendVarSetList, UniqSet.addListToUniqSet;
+  replace UniqSet.addOneToUniqSet with (fun x y => add y x) by auto.
+
+
+
+(* This tactic rewrites the boolean functions into the 
+   set properties to make them more suitable for fsetdec. *)
+
+Ltac set_b_iff :=
+  repeat
+   progress
+   rewrite <- not_mem_iff in *
+  || rewrite <- mem_iff in *
+  || rewrite <- subset_iff in *
+  || rewrite <- is_empty_iff in *
+  || rewrite delVarSet_remove in *
+  || rewrite extendVarSet_add in *
+  || rewrite empty_b in *
+  || rewrite unitVarSet_singleton in *
+  || rewrite_extendVarSetList
+  || rewrite delVarSetList_foldl in *.
+
+
+(*
+Hint Rewrite <- F.not_mem_iff : set_b.
+Hint Rewrite <- F.mem_iff : set_b.
+Hint Rewrite <- F.subset_iff : set_b.
+Hint Rewrite <- F.is_empty_iff : set_b.
+Hint Rewrite delVarSet_remove : set_b.
+Hint Rewrite extendVarSet_add : set_b.
+Hint Rewrite empty_b : set_b.
+*)
+
+(**************************************)
+
 (* Q: is there a way to do the automatic destructs safely? Sometimes 
    loses too much information. *)
+
+
 
 Ltac unfold_VarSet :=
   unfold subVarSet,elemVarSet, isEmptyVarSet, 
@@ -54,7 +155,7 @@ Ltac unfold_VarSet :=
   end;
   try repeat match goal with
   | u: UniqFM.UniqFM ?a |- context[match ?u with _ => _ end] => destruct u
-  end.
+  end. 
 
 Ltac safe_unfold_VarSet :=
   unfold subVarSet,elemVarSet, isEmptyVarSet, 
@@ -68,14 +169,12 @@ Ltac safe_unfold_VarSet :=
          UniqFM.minusUFM, UniqFM.isNullUFM, 
          UniqFM.elemUFM in *.
 
-
 Lemma extendVarSetList_nil:
   forall s,
   extendVarSetList s [] = s.
 Proof.
-  intro s. 
-  repeat unfold_VarSet.
-  unfold_Foldable_foldl'.
+  intro s.
+  set_b_iff.
   reflexivity.
 Qed.
 
@@ -84,7 +183,7 @@ Lemma extendVarSetList_cons:
   extendVarSetList s (v :: vs) = extendVarSetList (extendVarSet s v) vs.
 Proof.
   intros.
-  repeat unfold_VarSet.
+  set_b_iff.
   unfold_Foldable_foldl'.
   reflexivity.
 Qed.
@@ -96,16 +195,17 @@ Lemma extendVarSetList_append:
   extendVarSetList s (vs1 ++ vs2) = extendVarSetList (extendVarSetList s vs1) vs2.
 Proof.
   intros.
-  repeat unfold_VarSet.
+  set_b_iff.
   rewrite Foldable_foldl'_app.
   auto.
 Qed.
 
 Lemma elemVarSet_mkVarset_iff_In:
   forall v vs,
-  elemVarSet v (mkVarSet vs) = true <->  In (varUnique v) (map varUnique vs).
+  elemVarSet v (mkVarSet vs) = true <->  List.In (varUnique v) (map varUnique vs).
 Proof.
   intros.
+  set_b_iff.
   remember (mkVarSet vs) as vss.
   unfold_VarSet.
   rewrite <- getUnique_varUnique.
@@ -120,17 +220,13 @@ Lemma lookupVarSet_extendVarSet_self:
 Admitted.
 
 
+
 Lemma elemVarSet_extendVarSet:
   forall v vs v',
-  elemVarSet v (extendVarSet vs v') = (varUnique v == varUnique v') || elemVarSet v vs.
+  elemVarSet v (extendVarSet vs v') = (F.eqb v' v) || elemVarSet v vs.
 Proof.
   intros.
-  safe_unfold_VarSet.
-  destruct vs.
-  destruct u.
-  rewrite unique_word.
-  rewrite <- getUnique_varUnique.
-  apply member_insert.
+  eapply MP.Dec.F.add_b.
 Qed.
   
 Lemma subVarSet_refl:
@@ -138,23 +234,42 @@ Lemma subVarSet_refl:
   subVarSet vs1 vs1 = true.
 Proof.
   intros.
-  safe_unfold_VarSet.
-  destruct vs1.
-  destruct u.
-  rewrite difference_self.
-  apply null_empty.
+  set_b_iff.
+  fsetdec.
 Qed.
 
-Axiom elemVarSet_unitVarSet: forall v1 v2,
+Lemma elemVarSet_unitVarSet: forall v1 v2,
   (elemVarSet v1 (unitVarSet v2) = true) <-> (varUnique v1 = varUnique v2).
-Axiom elemVarSet_delVarSet: forall v1 fvs v2,
+Proof.
+  intros v1 v2.
+  set_b_iff.
+  rewrite singleton_iff.
+  unfold Var_as_DT.eqb.
+  unfold_zeze.
+Admitted.
+  
+
+Lemma elemVarSet_delVarSet: forall v1 fvs v2,
   elemVarSet v1 (delVarSet fvs v2) = true <-> (varUnique v1 <> varUnique v2 /\ elemVarSet v1 fvs = true).
-Axiom elemVarSet_false_true:
+Proof.
+  intros.
+  set_b_iff.
+  set_iff.
+  unfold Var_as_DT.eqb.
+  unfold_zeze.
+Admitted.
+
+Lemma elemVarSet_false_true:
   forall v1 fvs v2,
   elemVarSet v1 fvs = false ->
   elemVarSet v2 fvs = true ->
   varUnique v1 <> varUnique v2.
-
+Proof.
+  intros v1 fvs v2.
+  set_b_iff.
+  intros.
+Admitted.
+  
 
 Lemma subVarSet_elemVarSet_true:
   forall v vs vs',
@@ -162,40 +277,83 @@ Lemma subVarSet_elemVarSet_true:
   elemVarSet v vs = true ->
   elemVarSet v vs' = true.
 Proof.
-  intros.
-  safe_unfold_VarSet.
-  destruct vs.
-  destruct vs'.
-  destruct u.
-  destruct u0.
-  set (key := Unique.getWordKey (Unique.getUnique v)) in *.
-Admitted.
+  intros v vs vs'.
+  set_b_iff.
+  fsetdec.
+Qed.
 
-Axiom subVarSet_elemVarSet_false:
+Lemma subVarSet_elemVarSet_false:
   forall v vs vs',
   subVarSet vs vs' = true ->
   elemVarSet v vs' = false ->
   elemVarSet v vs = false.
+Proof.
+  intros v vs vs'.
+  set_b_iff.
+  fsetdec.
+Qed.
 
-Axiom subVarSet_extendVarSetList_l:
+Lemma subVarSet_extendVarSetList_l:
   forall vs1 vs2 vs,
   subVarSet vs1 vs2 = true ->
   subVarSet vs1 (extendVarSetList vs2 vs) = true.
+Proof.
+  intros vs1 vs2 vs.
+  generalize vs2. clear vs2.
+  induction vs.
+  - intro vs2. rewrite extendVarSetList_nil. auto.
+  - intro vs2. intro h. 
+    rewrite extendVarSetList_cons. 
+    rewrite IHvs. auto. 
+    set_b_iff. fsetdec.
+Qed.
 
-Axiom subVarSet_extendVarSetList_r:
-  forall vs1 vs2 vs,
+Lemma subVarSet_extendVarSetList_r:
+  forall vs vs1 vs2,
   subVarSet vs1 (mkVarSet vs) = true ->
   subVarSet vs1 (extendVarSetList vs2 vs) = true.
-
-
-Axiom subVarSet_extendVarSet:
+Proof.
+  intros vs. 
+  induction vs; intros vs1 vs2.
+  - set_b_iff.
+    unfold_Foldable_foldl'.
+    simpl.
+    fsetdec.
+  - intro h. 
+    rewrite mkVarSet_extendVarSetList in h.
+    rewrite extendVarSetList_cons in *.
+Admitted.
+    
+    
+Lemma subVarSet_extendVarSet:
   forall vs1 vs2 v,
   subVarSet vs1 vs2 = true ->
   subVarSet vs1 (extendVarSet vs2 v) = true.
+Proof.
+  intros.
+  set_b_iff.
+  fsetdec.
+Qed.
 
-Axiom subVarSet_delVarSetList:
-  forall vs1 vs2,
-  subVarSet (delVarSetList vs1 vs2) vs1 = true.
+
+Lemma subVarSet_delVarSetList:
+  forall vs1 vl,
+  subVarSet (delVarSetList vs1 vl) vs1 = true.
+Proof.
+  intros.
+  set_b_iff.
+  generalize vs1. clear vs1. induction vl.
+  - intros vs1. unfold_Foldable_foldl.
+    simpl.
+    fsetdec.
+  - intros vs1. revert IHvl.
+    unfold_Foldable_foldl.
+    simpl.
+    intro IH. 
+    rewrite IH with (vs1 := delVarSet vs1 a).
+    set_b_iff.
+    fsetdec.
+Qed.
 
 Axiom disjointVarSet_mkVarSet:
   forall vs1 vs2,
@@ -228,7 +386,7 @@ Proof.
   intros.
   unfold getInScopeVars.
   unfold extendInScopeSetList.
-  unfold_VarSet.
+  set_b_iff.
   destruct iss.
   unfold_Foldable_foldl'.
   unfold_Foldable_foldl.
@@ -262,4 +420,5 @@ Proof.
   unfold uniqAway'.
   unfold realUnique.
 Admitted.
+
 
